concurrency/node-replication/Linearize.i.dfy
@@ -1,0 +1,636 @@
+include "../framework/StateMachines.s.dfy"
+include "NRSpec.s.dfy"
+include "NRSimple.i.dfy"
+
+module NROne(nrifc: NRIfc) refines StateMachine(nrifc) {
+  type Variables = nrifc.NRState
+
+  predicate Init(s: Variables) { s == nrifc.init_state() }
+
+  predicate Next(s: Variables, s': Variables, op: ifc.Op) {
+    match op.input {
+      case ROp(readonly_op) =>
+        && op.output == nrifc.read(s, readonly_op)
+        && s' == s
+      case UOp(update_op) =>
+        && nrifc.update(s, update_op) == nrifc.UpdateResult(s', op.output)
+    }
+  }
+}
+
+module Behavior(ifc: Ifc, sm: StateMachine(ifc)) {
+  datatype Behavior =
+    | Stepped(s: sm.Variables, op: sm.ifc.Op, tail: Behavior)
+    | Inited(s: sm.Variables)
+  {
+    predicate WF() {
+      match this {
+        case Stepped(s', op, tail) =>
+          && tail.WF()
+          && sm.Next(tail.s, s', op)
+        case Inited(s) =>
+          && sm.Init(s)
+      }
+    }
+  }
+}
+
+module NRSimple_Refines_NRSingle(nrifc: NRIfc) {
+  import simple = NRSimple(nrifc)
+  import one = AsyncStateMachine(nrifc, NROne(nrifc))
+
+  import AI = AsyncIfc(nrifc)
+  import SimpleB = Behavior(AsyncIfc(nrifc), NRSimple(nrifc))
+  import OneB = Behavior(AsyncIfc(nrifc), AsyncStateMachine(nrifc, NROne(nrifc)))
+  import opened RequestIds
+
+  predicate equiv(a: SimpleB.Behavior, b: OneB.Behavior)
+  decreases a, b
+  {
+    || (a.Inited? && b.Inited?)
+    || (a.Stepped? && a.op.InternalOp? && equiv(a.tail, b))
+    || (b.Stepped? && b.op.InternalOp? && equiv(a, b.tail))
+    || (a.Stepped? && b.Stepped? && a.op == b.op && equiv(a.tail, b.tail))
+  }
+
+  /*
+  function IReqs(s: simple.Variables, r_points: map<RequestId, nat>)
+    : map<RequestId,     
+  {
+    map 
+  }
+  */
+
+  predicate FutureRidOk(s: simple.Variables, rid: RequestId, version: nat)
+  {
+    && rid in s.readonly_reqs
+    && (s.readonly_reqs[rid].ReadInit? ==>
+      s.ctail <= version
+    )
+    && (s.readonly_reqs[rid].ReadReq? ==>
+      s.readonly_reqs[rid].ctail_at_start <= version
+    )
+  }
+
+  predicate FuturePointsOk(s: simple.Variables, r_points: map<RequestId, nat>)
+  {
+    forall rid | rid in r_points :: FutureRidOk(s, rid, r_points[rid])
+  }
+
+  predicate readonly_is_req(
+      s: simple.Variables, t: one.Variables, r_points: map<RequestId, nat>,
+      rid: RequestId)
+  {
+    && rid in s.readonly_reqs
+    && rid in t.reqs
+    && t.reqs[rid] == nrifc.ROp(s.readonly_reqs[rid].op)
+    && (s.readonly_reqs[rid].ReadReq? ==>
+      && s.readonly_reqs[rid].ctail_at_start <= s.ctail
+    )
+    && (rid in r_points ==> (
+      && s.ctail <= r_points[rid]
+      && (s.readonly_reqs[rid].ReadReq? ==>
+        s.ctail < r_points[rid]
+      )
+    ))
+  }
+
+  predicate readonly_is_resp(
+      s: simple.Variables, t: one.Variables, r_points: map<RequestId, nat>,
+      rid: RequestId)
+  {
+    && rid in t.resps
+    && rid in s.readonly_reqs
+    && s.readonly_reqs[rid].ReadReq?
+    && s.readonly_reqs[rid].ctail_at_start <= s.ctail
+    && (rid in r_points ==> (
+      && s.readonly_reqs[rid].ctail_at_start <= r_points[rid] <= s.ctail
+      && 0 <= r_points[rid] <= |s.log|
+      && t.resps[rid] == nrifc.read(
+          simple.state_at_version(s.log, r_points[rid]),
+          s.readonly_reqs[rid].op)
+    ))
+  }
+
+  predicate update_is_done(
+      s: simple.Variables, t: one.Variables, r_points: map<RequestId, nat>,
+      rid: RequestId)
+  {
+    && rid in t.resps
+    && rid in s.update_resps
+    && 0 <= s.update_resps[rid].idx_in_log < |s.log|
+    && t.resps[rid] == nrifc.update(
+        simple.state_at_version(s.log, s.update_resps[rid].idx_in_log),
+        s.log[s.update_resps[rid].idx_in_log]
+     ).return_value
+  }
+
+  predicate rel(s: simple.Variables, t: one.Variables, r_points: map<RequestId, nat>)
+  {
+    && rel_basic(s, t, r_points)
+    && rel_r(s, t, r_points)
+  }
+
+  predicate HasVersion(update_resps: map<RequestId, simple.UpdateResp>, ver: int)
+  {
+    exists rid :: rid in update_resps && update_resps[rid].idx_in_log == ver
+  }
+
+  predicate rel_basic(s: simple.Variables, t: one.Variables, r_points: map<RequestId, nat>)
+  {
+    && 0 <= s.ctail <= |s.log|
+    && t.s == simple.state_at_version(s.log, s.ctail)
+    //&& t.reqs == IReqs(s, r_points)
+    //&& t.resps == IResps(s, r_points)
+    && (s.readonly_reqs.Keys !! s.update_reqs.Keys !! s.update_resps.Keys)
+    && (t.reqs.Keys !! t.resps.Keys)
+    && (forall rid ::
+        (rid in s.readonly_reqs || rid in s.update_reqs || rid in s.update_resps) <==>
+          (rid in t.reqs || rid in t.resps))
+    && (forall rid :: rid in t.reqs && t.reqs[rid].ROp? ==>
+            && rid in s.readonly_reqs
+    )
+    && (forall rid :: rid in t.reqs && t.reqs[rid].UOp? ==>
+            rid in s.update_reqs || rid in s.update_resps
+    )
+    && (forall rid :: rid in t.resps ==>
+            rid in s.readonly_reqs || rid in s.update_resps
+    )
+    && (forall ver | s.ctail <= ver < |s.log| :: HasVersion(s.update_resps, ver))
+    && (forall rid1, rid2 | rid1 in s.update_resps && rid2 in s.update_resps && rid1 != rid2 ::
+        s.update_resps[rid1] != s.update_resps[rid2])
+    && (forall rid | rid in s.update_resps ::
+            s.update_resps[rid].idx_in_log < |s.log|)
+
+    && (forall rid | rid in s.update_reqs ::
+            && rid in t.reqs
+            && t.reqs[rid] == nrifc.UOp(s.update_reqs[rid])
+    )
+
+    && (forall rid | rid in s.update_resps && (s.update_resps[rid].idx_in_log >= s.ctail) ::
+            && rid in t.reqs
+            && 0 <= s.update_resps[rid].idx_in_log < |s.log|
+            && t.reqs[rid] == nrifc.UOp(s.log[s.update_resps[rid].idx_in_log])
+    )
+
+    && (forall rid | rid in s.update_resps && (s.update_resps[rid].idx_in_log < s.ctail) ::
+      update_is_done(s, t, r_points, rid)
+    )
+  }
+
+  predicate rel_r(s: simple.Variables, t: one.Variables, r_points: map<RequestId, nat>)
+  {
+    && (forall rid | rid in s.readonly_reqs && rid in t.reqs ::
+      readonly_is_req(s, t, r_points, rid)
+    )
+
+    && (forall rid | rid in s.readonly_reqs && rid in t.resps ::
+      readonly_is_resp(s, t, r_points, rid)
+    )
+  }
+
+  lemma StartUpdate_Refines(s: simple.Variables, s': simple.Variables, Is: one.Variables,
+      r_points: map<RequestId, nat>,
+      rid: RequestId, uop: nrifc.UpdateOp)
+  returns (Is': one.Variables)
+  requires simple.StartUpdate(s, s', rid, uop)
+  requires rel(s, Is, r_points)
+  ensures rel(s', Is', r_points)
+  ensures one.Next(Is, Is', AI.Start(rid, nrifc.UOp(uop)))
+  {
+    Is' := Is.(reqs := Is.reqs[rid := nrifc.UOp(uop)]);
+  }
+
+  lemma state_at_version_preserves(a: seq<nrifc.UpdateOp>, b: seq<nrifc.UpdateOp>, x: seq<nrifc.UpdateOp>, i: nat)
+  requires b == a + x
+  requires 0 <= i <= |a|
+  requires 0 <= i <= |b|
+  ensures simple.state_at_version(a, i) == simple.state_at_version(b, i)
+  decreases i
+  {
+    if i > 0 {
+      state_at_version_preserves(a, b, x, i-1);
+    }
+  }
+
+  lemma AddUpdateToLog_Refines(s: simple.Variables, s': simple.Variables, Is: one.Variables,
+      r_points: map<RequestId, nat>,
+      request_ids: seq<RequestId>)
+  returns (Is': one.Variables)
+  requires simple.AddUpdateToLog(s, s', request_ids)
+  requires rel(s, Is, r_points)
+  ensures rel(s', Is', r_points)
+  ensures one.Next(Is, Is', AI.InternalOp)
+  {
+    Is' := Is;
+
+    var new_log_entries := simple.ConstructNewLogEntries(request_ids, s.update_reqs);
+    var new_responses := simple.ConstructUpdateResponses(request_ids, |s.log|);
+
+    state_at_version_preserves(s.log, s'.log, new_log_entries, s.ctail);
+
+    /*
+    forall rid
+    ensures rid in s.update_reqs ==> rid in s'.update_reqs || rid in s'.update_resps
+    ensures rid in s.update_resps ==> rid in s'.update_resps
+    ensures rid in s'.update_reqs ==> rid in s.update_reqs
+    ensures rid in s'.update_resps ==> rid in s.update_reqs || rid in s.update_resps
+    {
+      simple.reveal_map_filter();
+      simple.reveal_map_update();
+      simple.ConstructUpdateResponses_in_map(request_ids, |s.log|, new_responses);
+      if (rid in request_ids) {
+        if rid in s.update_reqs {
+          assert rid in s'.update_resps;
+        }
+        assert rid in s.update_reqs ==> rid in s'.update_reqs || rid in s'.update_resps;
+        assert rid in s.update_resps ==> rid in s'.update_resps;
+        assert rid in s'.update_reqs ==> rid in s.update_reqs;
+        assert rid in s'.update_resps ==> rid in s.update_reqs || rid in s.update_resps;
+      } else {
+        assert rid in s.update_reqs ==> rid in s'.update_reqs || rid in s'.update_resps;
+        assert rid in s.update_resps ==> rid in s'.update_resps;
+        assert rid in s'.update_reqs ==> rid in s.update_reqs;
+        assert rid in s'.update_resps ==> rid in s.update_reqs || rid in s.update_resps;
+      }
+    }
+
+    assert s'.update_reqs.Keys !! s'.update_resps.Keys
+    by {
+      simple.reveal_map_filter();
+      simple.reveal_map_update();
+      simple.ConstructUpdateResponses_in_map(request_ids, |s.log|, new_responses);
+    }
+    */
+
+    simple.reveal_map_filter();
+    simple.reveal_map_update();
+    simple.ConstructUpdateResponses_in_map(request_ids, |s.log|, new_responses);
+
+    /*forall rid | rid in s.readonly_reqs && rid in t.resps ::
+            && readonly_is_resp(s, t, r_points, rid)*/
+
+    forall rid | rid in s'.readonly_reqs && rid in Is'.resps
+    ensures readonly_is_resp(s', Is', r_points, rid)
+    {
+      if rid in r_points {
+        state_at_version_preserves(s.log, s'.log, new_log_entries, r_points[rid]);
+      }
+    }
+
+    forall rid | rid in s'.update_resps && (s'.update_resps[rid].idx_in_log < s'.ctail)
+    ensures update_is_done(s', Is', r_points, rid)
+    {
+      state_at_version_preserves(s.log, s'.log, new_log_entries,
+          s.update_resps[rid].idx_in_log);
+    }
+
+    forall ver | s'.ctail <= ver < |s'.log|
+    ensures HasVersion(s'.update_resps, ver)
+    {
+      if ver < |s'.log| - |new_log_entries| {
+        assert HasVersion(s.update_resps, ver);
+        var qid :| qid in s.update_resps && s.update_resps[qid].idx_in_log == ver;
+        assert s'.update_resps[qid].idx_in_log == ver;
+      } else {
+        var j := ver - (|s'.log| - |new_log_entries|);
+        assert s'.update_resps[request_ids[j]].idx_in_log == ver;
+      }
+    }
+    /*
+    forall rid1, rid2 | rid1 in s'.update_resps && rid2 in s'.update_resps && rid1 != rid2
+    ensures s'.update_resps[rid1] != s'.update_resps[rid2]
+    {
+      if s'.update_resps[rid1].idx_in_log < |s.log| {
+        if s'.update_resps[rid2].idx_in_log < |s.log| {
+          assert s'.update_resps[rid1] != s'.update_resps[rid2];
+        } else {
+          assert s'.update_resps[rid1] != s'.update_resps[rid2];
+        }
+      } else {
+        if s'.update_resps[rid2].idx_in_log < |s.log| {
+          assert s'.update_resps[rid1] != s'.update_resps[rid2];
+        } else {
+          assert s'.update_resps[rid1] != s'.update_resps[rid2];
+        }
+      }
+    }
+    */
+  }
+
+  lemma EndUpdate_Refines(s: simple.Variables, s': simple.Variables, Is: one.Variables,
+      r_points: map<RequestId, nat>,
+      rid: RequestId, return_value: nrifc.ReturnType)
+  returns (Is': one.Variables)
+  requires simple.EndUpdate(s, s', rid, return_value)
+  requires rel(s, Is, r_points)
+  ensures rel(s', Is', r_points)
+  ensures one.Next(Is, Is', AI.End(rid, return_value))
+  {
+    Is' := Is.(resps := Is.resps - {rid});
+
+    forall ver | s'.ctail <= ver < |s'.log|
+    ensures HasVersion(s'.update_resps, ver)
+    {
+      assert HasVersion(s.update_resps, ver);
+      var qid :| qid in s.update_resps && s.update_resps[qid].idx_in_log == ver;
+      assert s'.update_resps[qid].idx_in_log == ver;
+    }
+  }
+
+  lemma StartReadonly_Refines(s: simple.Variables, s': simple.Variables, Is: one.Variables,
+      r_points: map<RequestId, nat>,
+      rid: RequestId, rop: nrifc.ReadonlyOp)
+  returns (Is': one.Variables)
+  requires simple.StartReadonly(s, s', rid, rop)
+  requires rel(s, Is, r_points - {rid});
+  requires FuturePointsOk(s', r_points)
+  ensures rel(s', Is', r_points)
+  ensures one.Next(Is, Is', AI.Start(rid, nrifc.ROp(rop)))
+  {
+    Is' := Is.(reqs := Is.reqs[rid := nrifc.ROp(rop)]);
+
+    forall rid | rid in s'.readonly_reqs && rid in Is'.reqs
+    ensures readonly_is_req(s', Is', r_points, rid)
+    {
+    }
+  }
+
+  lemma ReadCtail_Refines(s: simple.Variables, s': simple.Variables, Is: one.Variables,
+      r_points: map<RequestId, nat>,
+      rid: RequestId)
+  returns (Is': one.Variables)
+  requires simple.ReadCtail(s, s', rid)
+  requires rel(s, Is, r_points);
+  requires FuturePointsOk(s', r_points)
+  ensures rel(s', Is', r_points)
+  ensures one.Next(Is, Is', AI.InternalOp)
+  {
+    if rid in r_points && r_points[rid] == s.ctail {
+      // linearization point is now
+      var retval := nrifc.read(
+            simple.state_at_version(s.log, r_points[rid]),
+            s.readonly_reqs[rid].op);
+      Is' := Is.(reqs := Is.reqs - {rid})
+               .(resps := Is.resps[rid := retval]);
+
+      var input := nrifc.ROp(s.readonly_reqs[rid].op);
+      assert one.InternalNext(rid, input, retval, Is, Is');
+
+      assert rel(s', Is', r_points);
+      assert one.Next(Is, Is', AI.InternalOp);
+    } else {
+      Is' := Is;
+
+      assert rel(s', Is', r_points);
+      assert one.Next(Is, Is', AI.InternalOp);
+    }
+  }
+
+  lemma FinishReadonly_Refines(s: simple.Variables, s': simple.Variables, Is: one.Variables,
+      r_points: map<RequestId, nat>,
+      rid: RequestId, version: nat, return_value: nrifc.ReturnType)
+  returns (Is': one.Variables)
+  requires simple.FinishReadonly(s, s', rid, version, return_value)
+  requires rel(s, Is, r_points[rid := version])
+  ensures rel(s', Is', r_points)
+  ensures one.Next(Is, Is', AI.End(rid, return_value))
+  {
+    Is' := Is.(resps := Is.resps - {rid});
+  }
+
+  function AllReadsFor(readonly_reqs: map<RequestId, simple.ReadReq>,
+    r_points: map<RequestId, nat>, ver: int) : set<RequestId>
+  {
+    set rid: RequestId | rid in r_points && r_points[rid] == ver
+        && rid in readonly_reqs && readonly_reqs[rid].ReadReq?
+  }
+
+  lemma pop_rid(t: set<RequestId>)
+  returns (t': set<RequestId>, r: RequestId)
+  requires t != {}
+  ensures |t'| < |t|
+  ensures r in t
+  ensures t' == t - {r}
+  {
+    r :| r in t;
+    t' := t - {r};
+    assert t == t' + {r};
+    assert |t| == |t'| + 1;
+  }
+
+  lemma {:induction true} trick_equiv(a: SimpleB.Behavior, a': SimpleB.Behavior, b: OneB.Behavior)
+  requires equiv(a, b)
+  requires a.Stepped? && a'.Stepped?
+  requires a.tail == a'.tail
+  requires a.op.InternalOp?
+  requires a'.op.InternalOp?
+  ensures equiv(a', b)
+  {
+  }
+
+  lemma IncCtail1(b: OneB.Behavior, a: SimpleB.Behavior, a': SimpleB.Behavior,
+      r_points: map<RequestId, nat>)
+  returns (b': OneB.Behavior)
+  requires a.WF()
+  requires FuturePointsOk(a'.s, r_points)
+  requires a.Stepped? && a'.Stepped?
+  requires a.tail == a'.tail
+  requires a.op.InternalOp?
+  requires a'.op.InternalOp?
+  requires a'.s == a.s.(ctail := a.s.ctail + 1)
+  requires a.s.ctail + 1 <= |a.s.log|
+  requires b.WF()
+  requires equiv(a, b)
+  requires rel(a.s, b.s, r_points)
+  ensures b'.WF()
+  ensures equiv(a', b')
+  ensures rel(a'.s, b'.s, r_points)
+  {
+    // Linearization point for the update
+
+    var s := a.s;
+    var s' := a'.s;
+
+    assert s.ctail < |s.log|;
+    assert HasVersion(s.update_resps, s.ctail);
+    var urid :| urid in s.update_resps && s.update_resps[urid].idx_in_log == s.ctail;
+
+    var x := nrifc.update(
+        simple.state_at_version(s.log, s.update_resps[urid].idx_in_log),
+        s.log[s.update_resps[urid].idx_in_log]
+     );
+    var uret := x.return_value;
+
+    var Is' := b.s
+        .(s := x.new_state)
+        .(reqs := b.s.reqs - {urid})
+        .(resps := b.s.resps[urid := uret]);
+    b' := OneB.Stepped(Is', AI.InternalOp, b);
+
+    var input := nrifc.UOp(s.log[s.update_resps[urid].idx_in_log]);
+    assert simple.state_at_version(s.log, s.update_resps[urid].idx_in_log) == b.s.s;
+    assert one.InternalNext(urid, input, uret, b.s, b'.s);
+    assert one.Next(b.s, b'.s, AI.InternalOp);
+
+    var the_reads := AllReadsFor(s.readonly_reqs, r_points, s.ctail + 1);
+
+    trick_equiv(a, a', b');
+
+    /*forall rid | rid in s.readonly_reqs && rid in b'.s.reqs && rid !in the_reads
+    ensures readonly_is_req(s', b'.s, r_points, rid)
+    {
+      if rid in r_points {
+        assert s.ctail <= r_points[rid];
+        assert r_points[rid] != s.ctail + 1;
+        assert s'.ctail == s.ctail + 1;
+        assert s'.ctail <= r_points[rid];
+      }
+    }*/
+
+    while the_reads != {}
+    decreases |the_reads|
+    invariant b'.WF()
+    invariant equiv(a', b')
+    invariant rel_basic(a'.s, b'.s, r_points)
+    invariant forall rid | rid in the_reads ::
+        && rid in r_points
+        && r_points[rid] == s.ctail + 1
+        && rid in s.readonly_reqs
+        && s.readonly_reqs[rid].ReadReq?
+    invariant (forall rid | rid in s.readonly_reqs && rid in b'.s.reqs ::
+      rid !in the_reads ==>
+      readonly_is_req(s', b'.s, r_points, rid)
+    )
+    invariant (forall rid | rid in s.readonly_reqs && rid in b'.s.resps ::
+      rid !in the_reads ==>
+      readonly_is_resp(s', b'.s, r_points, rid)
+    )
+    invariant (forall rid | rid in s.readonly_reqs && rid in b'.s.reqs ::
+      rid in the_reads ==>
+      readonly_is_req(s, b'.s, r_points, rid)
+    )
+    invariant (forall rid | rid in s.readonly_reqs && rid in b'.s.resps ::
+      rid in the_reads ==>
+      readonly_is_resp(s, b'.s, r_points, rid)
+    )
+    {
+      var the_reads', rid := pop_rid(the_reads);
+
+      var ret := nrifc.read(
+          simple.state_at_version(s.log, r_points[rid]),
+          s.readonly_reqs[rid].op);
+
+      var Is'' := b'.s
+          .(reqs := b'.s.reqs - {rid})
+          .(resps := b'.s.resps[rid := ret]);
+
+      var b'' := OneB.Stepped(Is'', AI.InternalOp, b');
+
+      var input := nrifc.ROp(s.readonly_reqs[rid].op);
+      assert one.InternalNext(rid, input, ret, b'.s, b''.s);
+      assert one.Next(b'.s, b''.s, AI.InternalOp);
+
+      if rid in s.readonly_reqs && rid in b''.s.resps && rid !in the_reads' {
+        assert readonly_is_resp(s', b''.s, r_points, rid);
+      }
+      forall rid | rid in s.readonly_reqs && rid in b''.s.resps && rid !in the_reads'
+      ensures readonly_is_resp(s', b''.s, r_points, rid)
+      {
+      }
+
+      the_reads := the_reads';
+      b' := b'';
+    }
+  }
+
+  lemma CtailRec(a: SimpleB.Behavior, r_points: map<RequestId, nat>,
+      new_ctail: nat)
+  returns (b: OneB.Behavior)
+  requires a.WF()
+  requires FuturePointsOk(a.s, r_points)
+  requires a.Stepped?
+  requires a.op.InternalOp?
+  requires simple.IncreaseCtail(a.tail.s, a.s, new_ctail)
+  ensures b.WF()
+  ensures equiv(a, b)
+  ensures rel(a.s, b.s, r_points)
+  decreases a.tail, 1, new_ctail
+  {
+    if new_ctail == a.tail.s.ctail {
+      b := ExistsEquivBehaviorRec(a.tail, r_points);
+      assert a.s == a.tail.s;
+    } else {
+      var amid := a.(s := a.s.(ctail := a.s.ctail - 1));
+      assert simple.NextStep(amid.tail.s, amid.s, AI.InternalOp, simple.IncreaseCtail_Step(new_ctail - 1));
+      var bmid := CtailRec(amid, r_points, new_ctail - 1);
+      b := IncCtail1(bmid, amid, a, r_points);
+    }
+  }
+
+  lemma ExistsEquivBehaviorRec(a: SimpleB.Behavior, r_points: map<RequestId, nat>)
+  returns (b: OneB.Behavior)
+  requires a.WF()
+  requires FuturePointsOk(a.s, r_points)
+  ensures b.WF()
+  ensures equiv(a, b)
+  ensures rel(a.s, b.s, r_points)
+  decreases a, 0, 0
+  {
+    match a {
+      case Inited(s) => {
+        b := OneB.Inited(one.Variables(nrifc.init_state(), map[], map[])); 
+      }
+      case Stepped(s', op, tail) => {
+        var step :| simple.NextStep(tail.s, s', op, step);
+        match step {
+          case StartUpdate_Step(rid: RequestId, uop: nrifc.UpdateOp) => {
+            var b0 := ExistsEquivBehaviorRec(tail, r_points);
+            var Is' := StartUpdate_Refines(tail.s, s', b0.s, r_points, rid, uop);
+            b := OneB.Stepped(Is', op, b0);
+          }
+          case AddUpdateToLog_Step(request_ids: seq<RequestId>) => {
+            var b0 := ExistsEquivBehaviorRec(tail, r_points);
+            var Is' := AddUpdateToLog_Refines(tail.s, s', b0.s, r_points, request_ids);
+            b := OneB.Stepped(Is', op, b0);
+          }
+          case EndUpdate_Step(rid: RequestId, return_value: nrifc.ReturnType) => {
+            var b0 := ExistsEquivBehaviorRec(tail, r_points);
+            var Is' := EndUpdate_Refines(tail.s, s', b0.s, r_points, rid, return_value);
+            b := OneB.Stepped(Is', op, b0);
+          }
+          case IncreaseCtail_Step(new_ctail: nat) => {
+            b := CtailRec(a, r_points, new_ctail);
+          }
+          case StartReadonly_Step(rid: RequestId, rop: nrifc.ReadonlyOp) => {
+            var b0 := ExistsEquivBehaviorRec(tail, r_points - {rid});
+            var Is' := StartReadonly_Refines(tail.s, s', b0.s, r_points, rid, rop);
+            b := OneB.Stepped(Is', op, b0);
+          }
+          case ReadCtail_Step(rid: RequestId) => {
+            var b0 := ExistsEquivBehaviorRec(tail, r_points);
+            var Is' := ReadCtail_Refines(tail.s, s', b0.s, r_points, rid);
+            b := OneB.Stepped(Is', op, b0);
+          }
+          case FinishReadonly_Step(rid: RequestId, version: nat, return_value: nrifc.ReturnType) => {
+            var b0 := ExistsEquivBehaviorRec(tail, r_points[rid := version]);
+            var Is' := FinishReadonly_Refines(tail.s, s', b0.s, r_points, rid, version, return_value);
+            b := OneB.Stepped(Is', op, b0);
+          }
+          case Stutter_Step => {
+            b := ExistsEquivBehaviorRec(tail, r_points);
+          }
+        }
+      }
+    }
+  }
+
+  lemma ExistsEquivBehavior(a: SimpleB.Behavior)
+  returns (b: OneB.Behavior)
+  requires a.WF()
+  ensures b.WF()
+  ensures equiv(a, b)
+  {
+    b := ExistsEquivBehaviorRec(a, map[]);
+  }
+}
